Added a typeclass for VELLVM integers.
Currently this just wraps the CompCert types so we don't need to
duplicate as much complex code.

src/coq/DynamicValues.v
@@ -110,241 +110,364 @@ Definition undef_i1  := DVALUE_Undef.
 Definition undef_i8  := DVALUE_Undef.
 Definition undef_i32 := DVALUE_Undef.
 Definition undef_i64 := DVALUE_Undef.
+Definition undef_int := DVALUE_Undef.
+
+
+Class VInt I : Type :=
+  {
+    (* Comparisons *)
+    eq : I -> I -> bool;
+    cmp : comparison -> I -> I -> bool;
+    cmpu : comparison -> I -> I -> bool;
+
+    (* Constants *)
+    bitwidth : nat;
+    zero : I;
+    one : I;
+
+    (* Arithmetic *)
+    add : I -> I -> I;
+    add_carry : I -> I -> I -> I;
+    add_overflow : I -> I -> I -> I;
+
+    sub : I -> I -> I;
+    sub_borrow : I -> I -> I -> I;
+    sub_overflow : I -> I -> I -> I;
+
+    mul : I -> I -> I;
+
+    divu : I -> I -> I;
+    divs : I -> I -> I;
+    modu : I -> I -> I;
+    mods : I -> I -> I;
+
+    shl : I -> I -> I;
+    shr : I -> I -> I;
+    shru : I -> I -> I;
+
+    negative : I -> I;
+
+    (* Logic *)
+    and : I -> I -> I;
+    or : I -> I -> I;
+    xor : I -> I -> I;
+
+    (* Bounds *)
+    min_signed : Z;
+    max_signed : Z;
+
+    (* Conversion *)
+    to_dvalue : I -> dvalue;
+    unsigned : I -> Z;
+    signed : I -> Z;
+
+    repr : Z -> I;
+  }.
+
+
+  Global Instance VInt1 : VInt Int1.int :=
+  {
+    (* Comparisons *)
+    eq := Int1.eq;
+    cmp := Int1.cmp;
+    cmpu := Int1.cmpu;
+
+    bitwidth := 1;
+
+    (* Constants *)
+    zero := Int1.zero;
+    one := Int1.one;    
+
+    (* Arithmetic *)
+    add := Int1.add;
+    add_carry := Int1.add_carry;
+    add_overflow := Int1.add_overflow;
+
+    sub := Int1.sub;
+    sub_borrow := Int1.sub_borrow;
+    sub_overflow := Int1.sub_overflow;
+
+    mul := Int1.mul;
+
+    divu := Int1.divu;
+    divs := Int1.divs;
+    modu := Int1.modu;
+    mods := Int1.mods;
+
+    shl := Int1.shl;
+    shr := Int1.shr;
+    shru := Int1.shru;
+
+    negative := Int1.negative;
+
+    (* Logic *)
+    and := Int1.and;
+    or := Int1.or;
+    xor := Int1.xor;
+
+    (* Bounds *)
+    min_signed := Int1.min_signed;
+    max_signed := Int1.max_signed;
+    
+    (* Conversion *)
+    to_dvalue := DVALUE_I1;
+    unsigned := Int1.unsigned;
+    signed := Int1.signed;
+
+    repr := Int1.repr;
+  }.
+
+
+  Global Instance VInt8 : VInt Int8.int :=
+  {
+    (* Comparisons *)
+    eq := Int8.eq;
+    cmp := Int8.cmp;
+    cmpu := Int8.cmpu;
+
+    bitwidth := 8;
+
+    (* Constants *)
+    zero := Int8.zero;
+    one := Int8.one;    
+
+    (* Arithmetic *)
+    add := Int8.add;
+    add_carry := Int8.add_carry;
+    add_overflow := Int8.add_overflow;
+
+    sub := Int8.sub;
+    sub_borrow := Int8.sub_borrow;
+    sub_overflow := Int8.sub_overflow;
+
+    mul := Int8.mul;
+
+    divu := Int8.divu;
+    divs := Int8.divs;
+    modu := Int8.modu;
+    mods := Int8.mods;
+
+    shl := Int8.shl;
+    shr := Int8.shr;
+    shru := Int8.shru;
+
+    negative := Int8.negative;
+
+    (* Logic *)
+    and := Int8.and;
+    or := Int8.or;
+    xor := Int8.xor;
+
+    (* Bounds *)
+    min_signed := Int8.min_signed;
+    max_signed := Int8.max_signed;
+    
+    (* Conversion *)
+    to_dvalue := DVALUE_I8;
+    unsigned := Int8.unsigned;
+    signed := Int8.signed;
+
+    repr := Int8.repr;
+  }.
+
+
+  Global Instance VInt32 : VInt Int32.int :=
+  {
+    (* Comparisons *)
+    eq := Int32.eq;
+    cmp := Int32.cmp;
+    cmpu := Int32.cmpu;
+
+    bitwidth := 32;
+
+    (* Constants *)
+    zero := Int32.zero;
+    one := Int32.one;    
+
+    (* Arithmetic *)
+    add := Int32.add;
+    add_carry := Int32.add_carry;
+    add_overflow := Int32.add_overflow;
+
+    sub := Int32.sub;
+    sub_borrow := Int32.sub_borrow;
+    sub_overflow := Int32.sub_overflow;
+
+    mul := Int32.mul;
+
+    divu := Int32.divu;
+    divs := Int32.divs;
+    modu := Int32.modu;
+    mods := Int32.mods;
+
+    shl := Int32.shl;
+    shr := Int32.shr;
+    shru := Int32.shru;
+
+    negative := Int32.negative;
+
+    (* Logic *)
+    and := Int32.and;
+    or := Int32.or;
+    xor := Int32.xor;
+
+    (* Bounds *)
+    min_signed := Int32.min_signed;
+    max_signed := Int32.max_signed;
+    
+    (* Conversion *)
+    to_dvalue := DVALUE_I32;
+    unsigned := Int32.unsigned;
+    signed := Int32.signed;
+
+    repr := Int32.repr;
+  }.
+
+  Global Instance VInt64 : VInt Int64.int :=
+  {
+    (* Comparisons *)
+    eq := Int64.eq;
+    cmp := Int64.cmp;
+    cmpu := Int64.cmpu;
+
+    bitwidth := 64;
+
+    (* Constants *)
+    zero := Int64.zero;
+    one := Int64.one;
+
+    (* Arithmetic *)
+    add := Int64.add;
+    add_carry := Int64.add_carry;
+    add_overflow := Int64.add_overflow;
+
+    sub := Int64.sub;
+    sub_borrow := Int64.sub_borrow;
+    sub_overflow := Int64.sub_overflow;
+
+    mul := Int64.mul;
+
+    divu := Int64.divu;
+    divs := Int64.divs;
+    modu := Int64.modu;
+    mods := Int64.mods;
+
+    shl := Int64.shl;
+    shr := Int64.shr;
+    shru := Int64.shru;
+
+    negative := Int64.negative;
+
+    (* Logic *)
+    and := Int64.and;
+    or := Int64.or;
+    xor := Int64.xor;
+
+    (* Bounds *)
+    min_signed := Int64.min_signed;
+    max_signed := Int64.max_signed;
+    
+    (* Conversion *)
+    to_dvalue := DVALUE_I64;
+    unsigned := Int64.unsigned;
+    signed := Int64.signed;
+
+    repr := Int64.repr;
+  }.
+
 
   (* Arithmetic Operations ---------------------------------------------------- *)
   Section ARITHMETIC.
-
+    
   (* Since modules are not first class, this code duplication
      will probably have to do. *)
-
-  Definition eval_i1_op (iop:ibinop) (x y:inttyp 1) : dvalue:=
+  Definition eval_int_op `{VInt Int} (iop:ibinop) (x y: Int) : dvalue:=
     (* See eval_i64_op for a few comments *)
     match iop with
     | Add nuw nsw =>
-      if orb (andb nuw (Int1.eq (Int1.add_carry x y Int1.zero) Int1.one))
-             (andb nsw (Int1.eq (Int1.add_overflow x y Int1.zero) Int1.one))
-      then DVALUE_Poison else DVALUE_I1 (Int1.add x y)
+      if orb (andb nuw (eq (add_carry x y zero) one))
+             (andb nsw (eq (add_overflow x y zero) one))
+      then DVALUE_Poison else to_dvalue (add x y)
     | Sub nuw nsw =>
-      if orb (andb nuw (Int1.eq (Int1.sub_borrow x y Int1.zero) Int1.one))
-             (andb nsw (Int1.eq (Int1.sub_overflow x y Int1.zero) Int1.one))
-      then DVALUE_Poison else DVALUE_I1 (Int1.sub x y)
+      if orb (andb nuw (eq (sub_borrow x y zero) one))
+             (andb nsw (eq (sub_overflow x y zero) one))
+      then DVALUE_Poison else to_dvalue (sub x y)
     | Mul nuw nsw =>
       (* I1 mul can't overflow, just based on the 4 possible multiplications. *)
-      DVALUE_I1 (Int1.mul x y)
+      if (bitwidth == 1)%nat then to_dvalue (mul x y)
+      else 
+        let res := mul x y in
+        let res_s' := (signed x) * (signed y) in
+        if orb (andb nuw ((unsigned x) * (unsigned y) >?
+                      unsigned res))
+             (andb nsw (orb (min_signed >? res_s')
+                            (res_s' >? max_signed)))
+      then DVALUE_Poison else to_dvalue res
     | Shl nuw nsw =>
-      if (Int1.unsigned y) >=? 1 then undef_i1 else DVALUE_I1 x
+      if (bitwidth == 1)%nat
+      then
+        if (unsigned y) >=? 1 then undef_int else to_dvalue x
+      else
+        let bz := Z.of_nat bitwidth in
+        let res := shl x y in
+        let res_u := unsigned res in
+        let res_u' := Z.shiftl (unsigned x) (unsigned y) in
+        if (unsigned y) >=? bz then undef_int
+        else if orb (andb nuw (res_u' >? res_u))
+                    (andb nsw (negb (Z.shiftr (unsigned x)
+                                              (bz - unsigned y)
+                                     =? (unsigned (negative res))
+                                        * (Z.pow 2 (unsigned y) - 1))))
+             then DVALUE_Poison else to_dvalue res
     | UDiv ex =>
-      if andb ex (negb ((Int1.unsigned x) mod (Int1.unsigned y) =? 0))
-      then DVALUE_Poison else DVALUE_I1 (Int1.divu x y)
+      if andb ex (negb ((unsigned x) mod (unsigned y) =? 0))
+      then DVALUE_Poison else to_dvalue (divu x y)
     | SDiv ex =>
       (* What does signed i1 mean? *)
-      if andb ex (negb (((Int1.signed x) mod (Int1.signed y)) =? 0))
-      then DVALUE_Poison else DVALUE_I1 (Int1.divs x y)
+      if andb ex (negb (((signed x) mod (signed y)) =? 0))
+      then DVALUE_Poison else to_dvalue (divs x y)
     | LShr ex =>
-      if (Int1.unsigned y) >=? 1 then undef_i1 else DVALUE_I1 x
+      if (bitwidth == 1)%nat
+      then
+        if (unsigned y) >=? 1 then undef_int else to_dvalue x
+      else
+        let bz := Z.of_nat bitwidth in
+        if (unsigned y) >=? bz then undef_int
+        else if andb ex (negb ((unsigned x)
+                                 mod (Z.pow 2 (unsigned y)) =? 0))
+             then DVALUE_Poison else to_dvalue (shru x y)
     | AShr ex =>
-      if (Int1.unsigned y) >=? 1 then undef_i1 else DVALUE_I1 x
+      if (bitwidth == 1)%nat
+      then
+        if (unsigned y) >=? 1 then undef_int else to_dvalue x
+      else
+        let bz := Z.of_nat bitwidth in
+        if (unsigned y) >=? bz then undef_int
+        else if andb ex (negb ((unsigned x)
+                                 mod (Z.pow 2 (unsigned y)) =? 0))
+             then DVALUE_Poison else to_dvalue (shr x y)
+
     | URem =>
-      DVALUE_I1 (Int1.modu x y)
+      to_dvalue (modu x y)
     | SRem =>
-      DVALUE_I1 (Int1.mods x y)
+      to_dvalue (mods x y)
     | And =>
-      DVALUE_I1 (Int1.and x y)
+      to_dvalue (and x y)
     | Or =>
-      DVALUE_I1 (Int1.or x y)
+      to_dvalue (or x y)
     | Xor =>
-      DVALUE_I1 (Int1.xor x y)
+      to_dvalue (xor x y)
     end.
-  Arguments eval_i1_op _ _ _ : simpl nomatch.
+  Arguments eval_int_op _ _ _ : simpl nomatch.
 
-
-  Definition eval_i8_op (iop:ibinop) (x y:inttyp 8) : dvalue:=
-    match iop with
-    | Add nuw nsw =>
-      if orb (andb nuw (Int8.eq (Int8.add_carry x y Int8.zero) Int8.one))
-             (andb nsw (Int8.eq (Int8.add_overflow x y Int8.zero) Int8.one))
-      then DVALUE_Poison else DVALUE_I8 (Int8.add x y)
-    | Sub nuw nsw =>
-      if orb (andb nuw (Int8.eq (Int8.sub_borrow x y Int8.zero) Int8.one))
-             (andb nsw (Int8.eq (Int8.sub_overflow x y Int8.zero) Int8.one))
-      then DVALUE_Poison else DVALUE_I8 (Int8.sub x y)
-    | Mul nuw nsw =>
-      let res := Int8.mul x y in
-      let res_s' := (Int8.signed x) * (Int8.signed y) in
-      if orb (andb nuw ((Int8.unsigned x) * (Int8.unsigned y) >?
-                      Int8.unsigned res))
-             (andb nsw (orb (Int8.min_signed >? res_s')
-                            (res_s' >? Int8.max_signed)))
-      then DVALUE_Poison else DVALUE_I8 res
-    | Shl nuw nsw =>
-      let res := Int8.shl x y in
-      let res_u := Int8.unsigned res in
-      let res_u' := Z.shiftl (Int8.unsigned x) (Int8.unsigned y) in
-      if (Int8.unsigned y) >=? 8 then undef_i8
-      else if orb (andb nuw (res_u' >? res_u))
-                  (andb nsw (negb (Z.shiftr (Int8.unsigned x)
-                                            (8 - Int8.unsigned y)
-                                   =? (Int8.unsigned (Int8.negative res))
-                                      * (Z.pow 2 (Int8.unsigned y) - 1))))
-      then DVALUE_Poison else DVALUE_I8 res
-    | UDiv ex =>
-      if andb ex (negb ((Int8.unsigned x) mod (Int8.unsigned y) =? 0))
-      then DVALUE_Poison else DVALUE_I8 (Int8.divu x y)
-    | SDiv ex =>
-      if andb ex (negb (((Int8.signed x) mod (Int8.signed y)) =? 0))
-      then DVALUE_Poison else DVALUE_I8 (Int8.divs x y)
-    | LShr ex =>
-      if (Int8.unsigned y) >=? 8 then undef_i8
-      else if andb ex (negb ((Int8.unsigned x)
-                               mod (Z.pow 2 (Int8.unsigned y)) =? 0))
-      then DVALUE_Poison else DVALUE_I8 (Int8.shru x y)
-    | AShr ex =>
-      if (Int8.unsigned y) >=? 8 then undef_i8
-      else if andb ex (negb ((Int8.unsigned x)
-                               mod (Z.pow 2 (Int8.unsigned y)) =? 0))
-      then DVALUE_Poison else DVALUE_I8 (Int8.shr x y)
-    | URem =>
-      DVALUE_I8 (Int8.modu x y)
-    | SRem =>
-      DVALUE_I8 (Int8.mods x y)
-    | And =>
-      DVALUE_I8 (Int8.and x y)
-    | Or =>
-      DVALUE_I8 (Int8.or x y)
-    | Xor =>
-      DVALUE_I8 (Int8.xor x y)
-    end.
-  Arguments eval_i8_op _ _ _ : simpl nomatch.
-
-
-  Definition eval_i32_op (iop:ibinop) (x y:inttyp 32) : dvalue:=
-    match iop with
-    | Add nuw nsw =>
-      if orb (andb nuw (Int32.eq (Int32.add_carry x y Int32.zero) Int32.one))
-             (andb nsw (Int32.eq (Int32.add_overflow x y Int32.zero) Int32.one))
-      then DVALUE_Poison else DVALUE_I32 (Int32.add x y)
-    | Sub nuw nsw =>
-      if orb (andb nuw (Int32.eq (Int32.sub_borrow x y Int32.zero) Int32.one))
-             (andb nsw (Int32.eq (Int32.sub_overflow x y Int32.zero) Int32.one))
-      then DVALUE_Poison else DVALUE_I32 (Int32.sub x y)
-    | Mul nuw nsw =>
-      let res := Int32.mul x y in
-      let res_s' := (Int32.signed x) * (Int32.signed y) in
-      if orb (andb nuw ((Int32.unsigned x) * (Int32.unsigned y) >?
-                      Int32.unsigned res))
-             (andb nsw (orb (Int32.min_signed >? res_s')
-                            (res_s' >? Int32.max_signed)))
-      then DVALUE_Poison else DVALUE_I32 res
-    | Shl nuw nsw =>
-      let res := Int32.shl x y in
-      let res_u := Int32.unsigned res in
-      let res_u' := Z.shiftl (Int32.unsigned x) (Int32.unsigned y) in
-      if (Int32.unsigned y) >=? 32 then undef_i32
-      else if orb (andb nuw (res_u' >? res_u))
-                  (andb nsw (negb (Z.shiftr (Int32.unsigned x)
-                                            (32 - Int32.unsigned y)
-                                   =? (Int32.unsigned (Int32.negative res))
-                                      * (Z.pow 2 (Int32.unsigned y) - 1))))
-      then DVALUE_Poison else DVALUE_I32 res
-    | UDiv ex =>
-      if andb ex (negb ((Int32.unsigned x) mod (Int32.unsigned y) =? 0))
-      then DVALUE_Poison else DVALUE_I32 (Int32.divu x y)
-    | SDiv ex =>
-      if andb ex (negb (((Int32.signed x) mod (Int32.signed y)) =? 0))
-      then DVALUE_Poison else DVALUE_I32 (Int32.divs x y)
-    | LShr ex =>
-      if (Int32.unsigned y) >=? 32 then undef_i32
-      else if andb ex (negb ((Int32.unsigned x)
-                               mod (Z.pow 2 (Int32.unsigned y)) =? 0))
-      then DVALUE_Poison else DVALUE_I32 (Int32.shru x y)
-    | AShr ex =>
-      if (Int32.unsigned y) >=? 32 then undef_i32
-      else if andb ex (negb ((Int32.unsigned x)
-                               mod (Z.pow 2 (Int32.unsigned y)) =? 0))
-      then DVALUE_Poison else DVALUE_I32 (Int32.shr x y)
-    | URem =>
-      DVALUE_I32 (Int32.modu x y)
-    | SRem =>
-      DVALUE_I32 (Int32.mods x y)
-    | And =>
-      DVALUE_I32 (Int32.and x y)
-    | Or =>
-      DVALUE_I32 (Int32.or x y)
-    | Xor =>
-      DVALUE_I32 (Int32.xor x y)
-    end.
-  Arguments eval_i32_op _ _ _ : simpl nomatch.
-
-
-  Definition eval_i64_op (iop:ibinop) (x y:inttyp 64) : dvalue:=
-    (* This needs to be tested *)
-    match iop with
-    (* Following to cases are probably right since they use CompCert *)
-    | Add nuw nsw =>
-      if orb (andb nuw (Int64.eq (Int64.add_carry x y Int64.zero) Int64.one))
-             (andb nsw (Int64.eq (Int64.add_overflow x y Int64.zero) Int64.one))
-      then DVALUE_Poison else DVALUE_I64 (Int64.add x y)
-    | Sub nuw nsw =>
-      if orb (andb nuw (Int64.eq (Int64.sub_borrow x y Int64.zero) Int64.one))
-             (andb nsw (Int64.eq (Int64.sub_overflow x y Int64.zero) Int64.one))
-      then DVALUE_Poison else DVALUE_I64 (Int64.sub x y)
-    | Mul nuw nsw =>
-      let res := Int64.mul x y in
-      let res_s' := (Int64.signed x) * (Int64.signed y) in
-      if orb (andb nuw ((Int64.unsigned x) * (Int64.unsigned y) >?
-                      Int64.unsigned res))
-             (andb nsw (orb (Int64.min_signed >? res_s')
-                            (res_s' >? Int64.max_signed)))
-      then DVALUE_Poison else DVALUE_I64 res
-    | Shl nuw nsw =>
-      let res := Int64.shl x y in
-      let res_u := Int64.unsigned res in
-      let res_u' := Z.shiftl (Int64.unsigned x) (Int64.unsigned y) in
-      (* Unsigned shift x right by 64 - y. If shifted x != sign bit * (2^y - 1),
-         then there is overflow. *)
-      if (Int64.unsigned y) >=? 64 then undef_i64
-      else if orb (andb nuw (res_u' >? res_u))
-                  (andb nsw (negb (Z.shiftr (Int64.unsigned x)
-                                            (64 - Int64.unsigned y)
-                                   =? (Int64.unsigned (Int64.negative res))
-                                      * (Z.pow 2 (Int64.unsigned y) - 1))))
-           then DVALUE_Poison else DVALUE_I64 res
-    | UDiv ex =>
-      if andb ex (negb ((Int64.unsigned x) mod (Int64.unsigned y) =? 0))
-      then DVALUE_Poison else DVALUE_I64 (Int64.divu x y)
-    | SDiv ex =>
-      if andb ex (negb (((Int64.signed x) mod (Int64.signed y)) =? 0))
-      then DVALUE_Poison else DVALUE_I64 (Int64.divs x y)
-    | LShr ex =>
-      if (Int64.unsigned y) >=? 64 then undef_i64
-      else if andb ex (negb ((Int64.unsigned x)
-                               mod (Z.pow 2 (Int64.unsigned y)) =? 0))
-      then DVALUE_Poison else DVALUE_I64 (Int64.shru x y)
-    | AShr ex =>
-      if (Int64.unsigned y) >=? 64 then undef_i64
-      else if andb ex (negb ((Int64.unsigned x)
-                               mod (Z.pow 2 (Int64.unsigned y)) =? 0))
-      then DVALUE_Poison else DVALUE_I64 (Int64.shr x y)
-    | URem =>
-      DVALUE_I64 (Int64.modu x y)
-    | SRem =>
-      DVALUE_I64 (Int64.mods x y)
-    | And =>
-      DVALUE_I64 (Int64.and x y)
-    | Or =>
-      DVALUE_I64 (Int64.or x y)
-    | Xor =>
-      DVALUE_I64 (Int64.xor x y)
-    end.
-  Arguments eval_i64_op _ _ _ : simpl nomatch.
 
   (* Evaluate the given iop on the given arguments according to the bitsize *)
   Definition integer_op (bits:Z) (iop:ibinop) (x y:inttyp bits) : err dvalue :=
     match bits, x, y with
-    | 1, x, y => mret (eval_i1_op iop x y)
-    | 8, x, y => mret (eval_i8_op iop x y)
-    | 32, x, y => mret (eval_i32_op iop x y)
-    | 64, x, y => mret (eval_i64_op iop x y)
+    | 1, x, y => mret (eval_int_op iop x y)
+    | 8, x, y => mret (eval_int_op iop x y)
+    | 32, x, y => mret (eval_int_op iop x y)
+    | 64, x, y => mret (eval_int_op iop x y)
     | _, _, _ => failwith "unsupported bitsize"
     end.
   Arguments integer_op _ _ _ _ : simpl nomatch.
@@ -353,10 +476,10 @@ Definition undef_i64 := DVALUE_Undef.
      Takes the integer modulo 2^bits. *)
   Definition coerce_integer_to_int (bits:Z) (i:Z) : err dvalue :=
     match bits with
-    | 1 => mret (DVALUE_I1 (Int1.repr i))
-    | 8 => mret (DVALUE_I8 (Int8.repr i))
-    | 32 => mret (DVALUE_I32 (Int32.repr i))
-    | 64 => mret (DVALUE_I64 (Int64.repr i))
+    | 1 => mret (DVALUE_I1 (repr i))
+    | 8 => mret (DVALUE_I8 (repr i))
+    | 32 => mret (DVALUE_I32 (repr i))
+    | 64 => mret (DVALUE_I64 (repr i))
     | _ => failwith "unsupported integer size"
     end.
   Arguments coerce_integer_to_int _ _ : simpl nomatch.
@@ -374,10 +497,10 @@ Definition undef_i64 := DVALUE_Undef.
      in order to prevent eval_iop from being recursive. *)
   Definition eval_iop_integer_h iop v1 v2 : err dvalue :=
     match v1, v2 with
-    | DVALUE_I1 i1, DVALUE_I1 i2 => integer_op 1 iop i1 i2
-    | DVALUE_I8 i1, DVALUE_I8 i2 => integer_op 8 iop i1 i2
-    | DVALUE_I32 i1, DVALUE_I32 i2 => integer_op 32 iop i1 i2
-    | DVALUE_I64 i1, DVALUE_I64 i2 => integer_op 64 iop i1 i2
+    | DVALUE_I1 i1, DVALUE_I1 i2 => mret (eval_int_op iop i1 i2)
+    | DVALUE_I8 i1, DVALUE_I8 i2 => mret (eval_int_op iop i1 i2)
+    | DVALUE_I32 i1, DVALUE_I32 i2 => mret (eval_int_op iop i1 i2)
+    | DVALUE_I64 i1, DVALUE_I64 i2 => mret (eval_int_op iop i1 i2)
     | _, _ => failwith "ill_typed-iop"
     end.
   Arguments eval_iop_integer_h _ _ _ : simpl nomatch.
@@ -395,86 +518,28 @@ Definition undef_i64 := DVALUE_Undef.
   Arguments eval_iop _ _ _ : simpl nomatch.
 
 
-  Definition eval_i1_icmp icmp x y : dvalue :=
+  Definition eval_int_icmp `{VInt Int} icmp (x y : Int) : dvalue :=
     if match icmp with
-       | Eq => Int1.cmp Ceq x y
-       | Ne => Int1.cmp Cne x y
-       | Ugt => Int1.cmpu Cgt x y
-       | Uge => Int1.cmpu Cge x y
-       | Ult => Int1.cmpu Clt x y
-       | Ule => Int1.cmpu Cle x y
-       | Sgt => Int1.cmp Cgt x y
-       | Sge => Int1.cmp Cge x y
-       | Slt => Int1.cmp Clt x y
-       | Sle => Int1.cmp Cle x y
+       | Eq => cmp Ceq x y
+       | Ne => cmp Cne x y
+       | Ugt => cmpu Cgt x y
+       | Uge => cmpu Cge x y
+       | Ult => cmpu Clt x y
+       | Ule => cmpu Cle x y
+       | Sgt => cmp Cgt x y
+       | Sge => cmp Cge x y
+       | Slt => cmp Clt x y
+       | Sle => cmp Cle x y
        end
-    then DVALUE_I1 Int1.one else DVALUE_I1 Int1.zero.
-  Arguments eval_i1_icmp _ _ _ : simpl nomatch.
-
-  Definition eval_i8_icmp icmp x y : dvalue :=
-    if match icmp with
-       | Eq => Int8.cmp Ceq x y
-       | Ne => Int8.cmp Cne x y
-       | Ugt => Int8.cmpu Cgt x y
-       | Uge => Int8.cmpu Cge x y
-       | Ult => Int8.cmpu Clt x y
-       | Ule => Int8.cmpu Cle x y
-       | Sgt => Int8.cmp Cgt x y
-       | Sge => Int8.cmp Cge x y
-       | Slt => Int8.cmp Clt x y
-       | Sle => Int8.cmp Cle x y
-       end
-    then DVALUE_I1 Int1.one else DVALUE_I1 Int1.zero.
-  Arguments eval_i8_icmp _ _ _ : simpl nomatch.
-
-  Definition eval_i32_icmp icmp x y : dvalue :=
-    if match icmp with
-       | Eq => Int32.cmp Ceq x y
-       | Ne => Int32.cmp Cne x y
-       | Ugt => Int32.cmpu Cgt x y
-       | Uge => Int32.cmpu Cge x y
-       | Ult => Int32.cmpu Clt x y
-       | Ule => Int32.cmpu Cle x y
-       | Sgt => Int32.cmp Cgt x y
-       | Sge => Int32.cmp Cge x y
-       | Slt => Int32.cmp Clt x y
-       | Sle => Int32.cmp Cle x y
-       end
-    then DVALUE_I1 Int1.one else DVALUE_I1 Int1.zero.
-  Arguments eval_i32_icmp _ _ _ : simpl nomatch.
-
-  Definition eval_i64_icmp icmp x y : dvalue :=
-    if match icmp with
-       | Eq => Int64.cmp Ceq x y
-       | Ne => Int64.cmp Cne x y
-       | Ugt => Int64.cmpu Cgt x y
-       | Uge => Int64.cmpu Cge x y
-       | Ult => Int64.cmpu Clt x y
-       | Ule => Int64.cmpu Cle x y
-       | Sgt => Int64.cmp Cgt x y
-       | Sge => Int64.cmp Cge x y
-       | Slt => Int64.cmp Clt x y
-       | Sle => Int64.cmp Cle x y
-       end
-    then DVALUE_I1 Int1.one else DVALUE_I1 Int1.zero.
-  Arguments eval_i64_icmp _ _ _ : simpl nomatch.
-
-  Definition integer_cmp bits icmp (x y:inttyp bits) : err dvalue :=
-    match bits, x, y with
-    | 1, x, y => mret (eval_i1_icmp icmp x y)
-    | 8, x, y => mret (eval_i8_icmp icmp x y)
-    | 32, x, y => mret (eval_i32_icmp icmp x y)
-    | 64, x, y => mret (eval_i64_icmp icmp x y)
-    | _, _, _ => failwith "unsupported bitsize"
-    end.
-  Arguments integer_cmp _ _ _ _ : simpl nomatch.
+    then to_dvalue one else to_dvalue zero.
+  Arguments eval_int_icmp _ _ _ : simpl nomatch.
 
   Definition eval_icmp icmp v1 v2 : err dvalue :=
     match v1, v2 with
-    | DVALUE_I1 i1, DVALUE_I1 i2 => integer_cmp 1 icmp i1 i2
-    | DVALUE_I8 i1, DVALUE_I8 i2 => integer_cmp 8 icmp i1 i2
-    | DVALUE_I32 i1, DVALUE_I32 i2 => integer_cmp 32 icmp i1 i2
-    | DVALUE_I64 i1, DVALUE_I64 i2 => integer_cmp 64 icmp i1 i2
+    | DVALUE_I1 i1, DVALUE_I1 i2 => mret (eval_int_icmp icmp i1 i2)
+    | DVALUE_I8 i1, DVALUE_I8 i2 => mret (eval_int_icmp icmp i1 i2)
+    | DVALUE_I32 i1, DVALUE_I32 i2 => mret (eval_int_icmp icmp i1 i2)
+    | DVALUE_I64 i1, DVALUE_I64 i2 => mret (eval_int_icmp icmp i1 i2)
     | _, _ => failwith "ill_typed-icmp"
     end.
   Arguments eval_icmp _ _ _ : simpl nomatch.
